Fixed issues with register update and jump

examples/sgx/Interpreter.fst
@@ -20,6 +20,15 @@ val STX.Store: unit -> buffer ... -> STX unit
 *)
 
 assume val search: (buffer dword)->(addr:address)-> bool
+val fold_left: ('a -> 'b -> STL 'a
+			(requires (fun h -> true))
+			(ensures (fun h0 r h1 -> true))) -> 'a -> list 'b -> STL 'a
+								(requires (fun h -> true))
+								(ensures (fun h0 r h1 -> true))
+let rec fold_left f x y = match y with
+  | [] -> x
+  | hd::tl -> fold_left f (f x hd) tl					
+
 
 type memaccess =
  |MkMemAccess: 
@@ -35,12 +44,20 @@ let defensive debugflag buf calltable base wbmapstart ucodestart uheapstart usta
   let read' (regname:string) (env:cpuregstate) :(Tot dword)  =
  	let rec search_reg (regname:string) (reglist:list register) :(Tot dword) = match reglist with
 		  |[] -> (* raise Halt *)
-			 let _ = if debugflag then debug_print_string "Bitmap not set: Raise Halt" else true in
+			 let _ = if debugflag then 
+					let _ = debug_print_string "Register " in
+					let _ = debug_print_string regname in
+					debug_print_string " not found: Raise Halt\n" else true in
 			 0uL
-		  |(MkReg regname' value)::tail -> if regname' = regname then
-								value
-							else
-								search_reg regname tail
+		  |(MkReg regname' value)::tail ->
+				 	let _ = if debugflag then 
+						let _ = debug_print_string "Register " in
+						let _ = debug_print_string regname' in
+						debug_print_string "\n" else true in
+					if regname' = regname then
+							value
+					else
+						search_reg regname tail
 	in
 	search_reg regname (get_reg_list env)
   in
@@ -132,10 +149,14 @@ val update: string -> dword->cpuregstate->Tot cpuregstate
 let update (regname:string) (value:dword) (env:cpuregstate) =
  let rec loop (pre:list register) (post:list register) :(Tot cpuregstate) = match post with
 	| [] -> (* raise Halt *) (Mkcpuregstate [])
-	| (MkReg regname' v)::tail -> if regname' = regname then
+	| (MkReg regname' v)::tail -> 
+						let _ = debug_print_string "Register " in
+						let _ = debug_print_string regname' in
+						let _ = debug_print_string "\n" in
+					if regname' = regname then
 						(Mkcpuregstate (pre@[MkReg regname value] @ tail))
 					  else
-						loop (pre@[(MkReg regname v)]) tail 
+						loop (pre@[(MkReg regname' v)]) tail 
 	in loop [] (get_reg_list env)
 						
 
@@ -156,22 +177,41 @@ val step : bool -> cpuregstate  ->memaccess-> program -> stmt -> STL cpuregstate
 val steps : bool-> cpuregstate ->memaccess-> program -> (list stmt) -> STL cpuregstate
 			(requires (fun h -> true))
 			(ensures (fun h0 r h1 -> true))
-assume val fold_right: ('a -> 'b -> STL 'b
-			(requires (fun h -> true))
-			(ensures (fun h0 r h1 -> true))) -> list 'a -> 'b -> STL 'b
-								(requires (fun h -> true))
-								(ensures (fun h0 r h1 -> true))
 let rec step (debugflag:bool) (env:cpuregstate) (defensivememop:memaccess) (myprogram:program) = function 
   | Skip iaddr ->
-       		let _ = if debugflag then
+       		let t = if debugflag then
 				debug_print_string "Skip;\n"
        			else true in
 		env
+  | Add (iaddr, ed, ea, eb) -> 
+        let op1 = eval env ea in
+        let op2 = eval env eb in 
+	let value = (add op1 op2) in
+        let regname = get_register_name ed in
+        let env' = update regname value env in
+        let t = if debugflag then
+		let _ = debug_print_string "Add " in
+		let _ = debug_print_string regname in
+		debug_print_string "\n"
+       		else true  in
+	 env'
+  | Cmp (iaddr, ed, ea, eb) -> 
+        let op1 = eval env ea in
+        let op2 = eval env eb in 
+	let value = if (eq op1 op2) then 1uL else 0uL in
+        let regname = get_register_name ed in
+        let env' = update regname value env in
+        let t = if debugflag then
+		let _ = debug_print_string "Cmp " in
+		let _ = debug_print_string regname in
+		debug_print_string "\n"
+       		else true  in
+	 env'
   | Store(iaddr, n, ea, ev)-> 
        let a = eval env ea in
        let v = eval env ev in 
        let _ = defensivememop.store (cast_to_word n) v a env in
-       let _ = if debugflag then
+       let t = if debugflag then
 			debug_print_string "Store;\n"
        		else true in
        env
@@ -181,8 +221,10 @@ let rec step (debugflag:bool) (env:cpuregstate) (defensivememop:memaccess) (mypr
        let value = defensivememop.load wordn a in
        let regname = get_register_name reg in
        let env' = update regname value env in
-       let _ = if debugflag then
-	debug_print_string "Load;\n"
+       let t = if debugflag then
+		let _ = debug_print_string "Load " in
+		let _ = debug_print_string regname in
+		debug_print_string "\n"
        else true  in
        env'
   | Call (iaddr, e) ->
@@ -191,16 +233,16 @@ let rec step (debugflag:bool) (env:cpuregstate) (defensivememop:memaccess) (mypr
 	   Raises Exception if the function is not callable 
 	*)	
        let  stmtlist = defensivememop.decode true myprogram fentry in
-       let _ = if debugflag then
+       let t = if debugflag then
 	debug_print_string "Call;\n"
        else true in
 	steps debugflag env defensivememop myprogram stmtlist 
   | If (iaddr, e, truli, falsli) ->
 	let boolval = eval env e in
-        let _ = if debugflag then
+        let t = if debugflag then
 			debug_print_string "If-Else;\n"
        		else true in
-	if not (eq boolval 0uL)  then
+	if not (eq boolval 1uL)  then
 		steps debugflag env defensivememop myprogram (invert_stmt truli)
 	else
 		steps debugflag env defensivememop myprogram (invert_stmt falsli) 
@@ -208,8 +250,10 @@ let rec step (debugflag:bool) (env:cpuregstate) (defensivememop:memaccess) (mypr
 	let value = eval env e in
         let regname = get_register_name reg in
         let env' = update regname value env in
-        let _ = if debugflag then
-		debug_print_string "Assign ;\n"
+        let t = if debugflag then
+		let _ = debug_print_string "Assign " in
+		let _ = debug_print_string regname in
+		debug_print_string "\n"
        		else true  in
 	 env'
 
@@ -218,9 +262,9 @@ let rec step (debugflag:bool) (env:cpuregstate) (defensivememop:memaccess) (mypr
 	let targetaddress = eval env e in
 	(* not modeling "rip" explicitly *)
 	(* Get the stmt list from updated "rip" *)
-        let  stmtlist = defensivememop.decode true myprogram targetaddress in
+        let  stmtlist = defensivememop.decode false myprogram targetaddress in
 	
-       let _ = if debugflag then
+       let t = if debugflag then
 	debug_print_string "Jump;\n"
        else  true in
 	steps debugflag env defensivememop myprogram stmtlist 
@@ -228,17 +272,17 @@ let rec step (debugflag:bool) (env:cpuregstate) (defensivememop:memaccess) (mypr
  | Return iaddr -> 
 	     let rspvalue = eval env (Register "rsp") in
 	     let rspvalue' = (sub rspvalue 1uL) in
-	      let _ =  if debugflag then
+	      let t =  if debugflag then
 		debug_print_string "Return;\n"
 	       else true in
 	     update "rsp" rspvalue' env
 
-and helperfunc  (debugflag:bool) (defensivememop:memaccess) (myprogram:program) (elem:stmt) (env':cpuregstate): STL cpuregstate 
+and helperfunc  (debugflag:bool) (defensivememop:memaccess) (myprogram:program) (env':cpuregstate) (elem:stmt): STL cpuregstate 
 					(requires (fun h -> true))
 					(ensures (fun h0 r h1 -> false)) =
 					step debugflag env' defensivememop myprogram elem 
 
-and steps (debugflag:bool) (env:cpuregstate) (defensivememop:memaccess) myprogram instrlist = fold_right   (helperfunc debugflag defensivememop myprogram) instrlist env  
+and steps (debugflag:bool) (env:cpuregstate) (defensivememop:memaccess) myprogram instrlist = fold_left (helperfunc debugflag defensivememop myprogram) env  instrlist 
 
 (* Should the following function have a type that uses effects associated with effect ST ?  *)
 val ustar:bool->(buffer dword)->(buffer dword)->address ->address->address->address->address->address->program->STL cpuregstate
@@ -246,7 +290,7 @@ val ustar:bool->(buffer dword)->(buffer dword)->address ->address->address->addr
 	(ensures (fun h0 r h1 -> True))
 let ustar debugflag buf calltable base wbmapstart uheapstart ustackstart ucodestart entry myprogram = 
   (* Modeling registers as list?? *)
-  let regslist = [MkReg "rsp" 0uL; MkReg "rbp" 0uL; MkReg "rip"  0uL; MkReg "rax" 0uL] in
+  let regslist = [MkReg "rsp" 0uL; MkReg "rbp" 0uL; MkReg "rax"  0uL; MkReg "rbx" 0uL; MkReg "rcx" 0uL] in
   let mem = defensive debugflag buf calltable base wbmapstart ucodestart uheapstart ustackstart in
   let stmtlist = mem.decode true  myprogram entry in
   let _ = if debugflag then debug_print_string "Stepping into main\n" else true in
